Progress on log'

composition/log.fst
@@ -3,7 +3,13 @@ open FStar.List.Tot
 
 open Library
 
-val mem_id_s : id:nat -> l:list (nat * string) -> Tot (b:bool {b = true <==> (exists m. mem (id,m) l)})
+  val fst : e:(nat * string) -> Tot (id:nat {exists m. e = (id, m)})
+    let fst (id, m) = id
+
+    val snd : e:(nat * string) -> Tot (m:string {exists id. e = (id, m)})
+    let snd (id, m) = m
+    
+val mem_id_s : id:nat -> l:list (nat * string) -> Tot (b:bool {b = true <==> (exists m. mem (id,m) l) /\ (exists e. mem e l ==> fst e = id)})
 let rec mem_id_s id l =
   match l with
   |[] -> false
@@ -15,28 +21,43 @@ let rec unique_s l =
   |[] -> true
   |(id,m)::xs -> not (mem_id_s id xs) && unique_s xs
 
+ 
+
+  val pos : id:(nat * string) -> l:list (nat * string) {mem id l /\ unique_s l} -> Tot nat
+    let rec pos id l =
+      match l with
+      |id1::xs -> if id = id1 then 0 else 1 + pos id xs
+
 val total_order : l:list (nat * string) {unique_s l}
                 -> Tot (b:bool)
 let rec total_order l =
   match l with
   |[] -> true
-  |[(id,m)] -> true
-  |(id, m)::(id1, m1)::xs -> id > id1 && total_order ((id1, m1)::xs)
+  |[x] -> true
+  |x::xs -> forallb (fun e -> fst x > fst e) xs && total_order xs
 
-  val pos : id:(nat * string) -> l:list (nat * string) {mem id l /\ unique_s l /\ total_order l} -> Tot nat
-  let rec pos id l =
-    match l with
-    |id1::xs -> if id = id1 then 0 else 1 + pos id xs
-
+val test_sorted: x:(nat * string) -> l:list (nat * string) ->
+                   Lemma ((unique_s (x::l) /\ total_order (x::l) /\ Cons? l) ==> fst x > fst (Cons?.hd l))
+let test_sorted x l = ()
 
 val ord : id:(nat * string)
-          -> id1:(nat * string)
-          -> l:list (nat * string)
-          -> Pure bool
-            (requires fst id <> fst id1 /\ mem id l /\ mem id1 l /\ unique_s l /\ total_order l)
-            (ensures (fun b -> b = true <==> pos id l < pos id1 l))
+            -> id1:(nat * string)
+            -> l:list (nat * string)
+            -> Pure bool
+              (requires fst id <> fst id1 /\ mem id l /\ mem id1 l /\ unique_s l /\ total_order l)
+              (ensures (fun b -> b = true <==> pos id l < pos id1 l))
 let ord id id1 l = pos id l < pos id1 l 
 
+val sorted_smaller: x:(nat * string)
+                      ->  y:(nat * string)
+                      ->  l:list (nat * string)
+                      ->  Lemma (requires (unique_s (x::l) /\ total_order (x::l) /\ mem y l))
+                                (ensures (fst x > fst y) /\ ord x y (x::l))
+                                [SMTPat (unique_s (x::l) /\ total_order (x::l))]
+let rec sorted_smaller x y l = match l with
+      | [] -> ()
+      | z::zs -> if z=y then () else sorted_smaller x y zs
+      
 type s = l: list (nat (*id*) * string (*message*)) {unique_s l /\ total_order l}
 
 type op =
@@ -48,25 +69,29 @@ let get_msg (id, (Append m)) = m
 val get_id : op1:(nat * op) -> Tot (id:nat {exists m. op1 = (id, (Append m))}) 
 let get_id (id, (Append m)) = id
 
-val fst : e:(nat * string) -> Tot (id:nat {exists m. e = (id, m)})
-let fst (id, m) = id
-
-val snd : e:(nat * string) -> Tot (m:string {exists id. e = (id, m)})
-let snd (id, m) = m
 
 val app_op : s1:s 
            -> op1:(nat * op)
            -> Pure s 
              (requires not (mem_id_s (get_id op1) s1) /\ (forall id. mem_id_s id s1 ==> get_id op1 > id))
-             (ensures (fun r -> (forall e. mem e r <==> mem e s1 \/ e = (get_id op1, get_msg op1))))
+             (ensures (fun r -> (forall e. mem e r <==> mem e s1 \/ e = (get_id op1, get_msg op1)) /\
+                             (forall e e1. mem e s1 /\ mem e1 s1 /\ fst e <> fst e1 /\ fst e > fst e1 /\ ord e e1 s1 <==>
+                                      mem e r /\ mem e1 r /\ fst e <> fst e1 /\ fst e > fst e1 /\
+                             e <> (get_id op1, get_msg op1) /\ e1 <> (get_id op1, get_msg op1) /\ ord e e1 r)))
+#set-options "--z3rlimit 1000000"
 let app_op s1 (id, (Append m)) = (id, m)::s1
 
 val filter_uni : f:((nat * string) -> bool)
                  -> l:list (nat * string) 
                  -> Lemma (requires (unique_s l /\ total_order l))
-                          (ensures (unique_s (filter f l) /\ total_order (filter f l)))
+                          (ensures (unique_s (filter f l) /\ total_order (filter f l)) /\
+                            (forall e. mem e l /\ f e <==> mem e (filter f l)) /\
+                            (forall e e1. mem e l /\ mem e1 l /\ fst e <> fst e1 /\ fst e > fst e1 /\ ord e e1 l /\ f e /\ f e1 <==>
+                     mem e (filter f l) /\ mem e1 (filter f l) /\ fst e <> fst e1 /\ fst e > fst e1 /\ ord e e1 (filter f l)))
                           [SMTPat (filter f l)]
-let rec filter_uni f l = admit();
+
+#set-options "--z3rlimit 1000000"
+let rec filter_uni f l =
     match l with
     |[] -> ()
     |x::xs -> filter_uni f xs
@@ -91,23 +116,19 @@ val sim : tr:ae op
         -> Tot (b:bool {b = true <==> (forall e. mem e s1 <==> mem (fst e, (Append (snd e))) tr.l) /\
                                    (forall e e1. mem e s1 /\ mem e1 s1 /\ fst e <> fst e1 /\ fst e > fst e1 /\ ord e e1 s1 <==>
                                       (mem (fst e, (Append (snd e))) tr.l /\ mem (fst e1, (Append (snd e1))) tr.l /\
-               fst e <> fst e1 /\ fst e > fst e1 /\ tr.vis (fst e1, (Append (snd e1))) (fst e, (Append (snd e)))) \/
-                   (mem (fst e, (Append (snd e))) tr.l /\ mem (fst e1, (Append (snd e1))) tr.l /\
-                   not (tr.vis (fst e1, (Append (snd e1))) (fst e, (Append (snd e))) ||
-              tr.vis (fst e, (Append (snd e))) (fst e1, (Append (snd e1)))) /\ fst e <> fst e1 /\ fst e > fst e1))})
+               fst e <> fst e1 /\ fst e > fst e1 (*)/\ (tr.vis (fst e1, (Append (snd e1))) (fst e, (Append (snd e))) \/
+               not (tr.vis (fst e1, (Append (snd e1))) (fst e, (Append (snd e))) ||
+               tr.vis (fst e, (Append (snd e))) (fst e1, (Append (snd e1))))*)))})
 
 #set-options "--z3rlimit 1000000"
-let sim tr s1 =
+let sim tr s1 = 
   forallb (fun e -> mem (fst e, (Append (snd e))) tr.l) s1 &&
   forallb (fun e -> mem (get_id e, get_msg e) s1) tr.l &&
   forallb (fun e -> (forallb (fun e1 -> (mem (fst e, (Append (snd e))) tr.l && mem (fst e1, (Append (snd e1))) tr.l &&
-              fst e <> fst e1 && fst e > fst e1 && tr.vis (fst e1, (Append (snd e1))) (fst e, (Append (snd e)))) ||
-             (not (tr.vis (fst e1, (Append (snd e1))) (fst e, (Append (snd e))) ||
-               tr.vis (fst e, (Append (snd e))) (fst e1, (Append (snd e1)))) && fst e <> fst e1 && fst e > fst e1)) 
+              fst e <> fst e1 && fst e > fst e1)) 
   (filter (fun e1 -> mem e1 s1 && mem e s1 && fst e <> fst e1 && fst e > fst e1 && ord e e1 s1) s1))) s1 &&
   forallb (fun e -> (forallb (fun e1 -> mem (get_id e, get_msg e) s1 && mem (get_id e1, get_msg e1) s1 && get_id e <> get_id e1 && get_id e > get_id e1 && ord (get_id e, get_msg e) (get_id e1, get_msg e1) s1)
-          (filter (fun e1 -> (get_id e <> get_id e1 && get_id e > get_id e1 && tr.vis e1 e) ||
-              (not (tr.vis e e1 || tr.vis e1 e) && get_id e <> get_id e1 && get_id e > get_id e1)) tr.l))) tr.l
+          (filter (fun e1 -> (get_id e <> get_id e1 && get_id e > get_id e1)) tr.l))) tr.l
 
 val prop_oper : tr:ae op
               -> st:s
@@ -115,20 +136,21 @@ val prop_oper : tr:ae op
               -> Lemma (requires (sim tr st) /\ (forall id. mem_id_s id st ==> get_id op > id) /\
                                 (not (member (get_id op) tr.l)))
                       (ensures (sim (append tr op) (app_op st op)))
+
+#set-options "--z3rlimit 1000000"
 let prop_oper tr st op = ()
 
 val remove_st : ele:(nat * string) -> a:s
                   -> Pure s
                     (requires (mem ele a))
-                    (ensures (fun r -> (forall e. mem e r <==> mem e a /\ e <> ele) /\
-                                    (forall id. mem_id_s id r <==> mem_id_s id a /\ id <> fst ele) /\
+                    (ensures (fun r -> (forall e. mem e r <==> mem e a /\ e <> ele) (*)/\
+                                    (forall id. mem_id_s id r <==> mem_id_s id a /\ id <> fst ele*) /\
                                     (forall e e1. mem e r /\ mem e1 r /\ fst e <> fst e1 /\ ord e e1 r /\ fst e > fst e1 <==>
-                                            mem e a /\ mem e1 a /\ fst e <> fst e1 /\ e <> ele /\ e1 <> ele /\ fst e > fst e1 /\ ord e e1 a) /\ List.Tot.length r = List.Tot.length a - 1))
-#set-options "--z3rlimit 10000"
-let rec remove_st ele a = admit();
-      match a with
-      |ele1::xs -> if ele = ele1 then xs 
-                   else ((assume (forall e. mem e xs ==> fst ele1 > fst e)); ele1::(remove_st ele xs))
+                         mem e a /\ mem e1 a /\ fst e <> fst e1 /\ e <> ele /\ e1 <> ele /\ fst e > fst e1 /\ ord e e1 a) (*)/\
+                                            List.Tot.length r = List.Tot.length a - 1*) ))
+
+#set-options "--z3rlimit 1000000"
+let rec remove_st ele a = filter (fun e -> e <> ele) a
 
 val convergence : tr:ae op
                     -> a:s
@@ -137,19 +159,60 @@ val convergence : tr:ae op
                             (ensures (forall id. mem_id_s id a <==> mem_id_s id b) /\ (forall e. mem e a <==> mem e b) /\
                                      (forall e e1. mem e a /\ mem e1 a /\ fst e <> fst e1 /\ ord e e1 a /\ fst e > fst e1 <==> 
                                               mem e b /\ mem e1 b /\ fst e <> fst e1 /\ ord e e1 b /\ fst e > fst e1))
-                            [SMTPat (sim tr a /\ sim tr b)]
+                            (*)[SMTPat (sim tr a /\ sim tr b)]*)
 let convergence tr a b = ()
+
+(*)val help : a:s 
+         -> Lemma (ensures (forall e e1. mem e a /\ mem e1 a /\ fst e <> fst e1 /\ fst e > fst e1 ==>
+                                   fst e <> fst e1 /\ mem e a /\ mem e1 a /\ ord e e1 a))
+                                   [SMTPat (unique_s a /\ total_order a)]
+
+#set-options "--z3rlimit 10000000"
+let rec help a = admit ();
+  match a with
+  |[] -> ()
+  |x::xs -> help xs*)
+
 
 val merge1 : l:s -> a:s -> b:s
            -> Pure s
-             (requires true)
+             (requires (forall e. mem e l ==> mem e a /\ mem e b) /\
+                       (forall e e1. mem e a /\ not (mem e l) /\ mem e1 b /\ not (mem e1 l) ==> e <> e1))
              (ensures (fun r -> (forall e. mem e r <==> mem e a \/ mem e b) /\
                              (forall e e1. mem e r /\ mem e1 r /\ fst e <> fst e1 /\ fst e > fst e1 /\ ord e e1 r <==>
                                      (mem e a /\ mem e1 a /\ fst e <> fst e1 /\ fst e > fst e1 /\ ord e e1 a) \/
                                      (mem e b /\ mem e1 b /\ fst e <> fst e1 /\ fst e > fst e1 /\ ord e e1 b) \/
                                      (mem e a /\ mem e1 b /\ fst e <> fst e1 /\ fst e > fst e1) \/
                                      (mem e b /\ mem e1 a /\ fst e <> fst e1 /\ fst e > fst e1))))
-let merge1 l a b = admit()
+                                     (decreases %[l;a;b])
+
+#set-options "--z3rlimit 10000000"
+let rec merge1 l a b = admit()
+
+val un : a:s -> b:s
+       -> Pure s
+         (requires (forall id. mem_id_s id a ==> not (mem_id_s id b)) /\
+                   (forall e e1. mem e a /\ mem e1 b ==> fst e <> fst e1))
+         (ensures (fun r -> (forall e. mem e r <==> mem e a \/ mem e b) /\
+                         (forall e e1. 
+                                      (mem e a /\ mem e1 a /\ fst e <> fst e1 /\ fst e > fst e1 /\ ord e e1 a) \/
+                                      (mem e b /\ mem e1 b /\ fst e <> fst e1 /\ fst e > fst e1 /\ ord e e1 b) \/
+                                      (mem e a /\ mem e1 b /\ fst e <> fst e1 /\ fst e > fst e1) \/
+                                      (mem e b /\ mem e1 a /\ fst e <> fst e1 /\ fst e > fst e1) ==>
+                                      mem e r /\ mem e1 r /\ fst e <> fst e1 /\ fst e > fst e1 /\ ord e e1 r)))
+
+#set-options "--z3rlimit 1000000"
+let rec un a b =
+  match a, b with
+  |[],[] -> []
+  |[],_ -> b
+  |x::xs,[] -> a 
+  |x::xs, y::ys -> if fst x > fst y then 
+                ((*)assume (forall e e1. mem e xs /\ mem e1 b ==> fst x > fst e /\ fst x > fst e1 /\ ord x e (x::(un xs b)) /\ 
+                        ord x e1 (x::(un xs b)));*)
+                       admit (); x::(un xs b)) else 
+                ((*)assume (forall e e1. mem e ys /\ mem e1 a ==> fst y > fst e /\ fst y > fst e1 /\ ord y e (y::(un a ys)) /\ 
+                         ord y e1 (y::(un a ys)));*)admit(); y::(un a ys))
 
 val merge : ltr:ae op
           -> l:s
@@ -163,39 +226,36 @@ val merge : ltr:ae op
                              (forall e e1. mem e ltr.l /\ mem e1 atr.l ==> get_id e < get_id e1) /\
                              (forall e e1. mem e ltr.l /\ mem e1 btr.l ==> get_id e < get_id e1) /\
                              (sim ltr l /\ sim (union ltr atr) a /\ sim (union ltr btr) b))
-                   (ensures (fun res -> res = merge1 l a b))
+                   (ensures (fun r -> (forall e. mem e r <==> mem e a \/ mem e b) /\
+                               (forall e e1. mem e r /\ mem e1 r /\ fst e <> fst e1 /\ fst e > fst e1 /\ ord e e1 r <==>
+                                        (mem e a /\ mem e1 a /\ fst e <> fst e1 /\ fst e > fst e1 /\ ord e e1 a) \/
+                                        (mem e b /\ mem e1 b /\ fst e <> fst e1 /\ fst e > fst e1 /\ ord e e1 b) \/
+                                        (mem e a /\ mem e1 b /\ fst e <> fst e1 /\ fst e > fst e1) \/
+                                        (mem e b /\ mem e1 a /\ fst e <> fst e1 /\ fst e > fst e1))
+                               (*forall e e1. mem e r /\ mem e1 r /\ fst e <> fst e1 /\ fst e > fst e1 /\ ord e e1 r <==>
+                            (mem e l /\ mem e1 l /\ fst e <> fst e1 /\ fst e > fst e1 /\ ord e e1 l) \/
+                            (mem e (diff a l) /\ mem e1 (diff a l) /\ fst e <> fst e1 /\ fst e > fst e1 /\ ord e e1 (diff a l)) \/
+                            (mem e (diff b l) /\ mem e1 (diff b l) /\ fst e <> fst e1 /\ fst e > fst e1 /\ ord e e1 (diff b l)) \/
+                            (mem e (diff a l) /\ mem e1 l /\ fst e <> fst e1 /\ fst e > fst e1) \/
+                            (mem e (diff b l) /\ mem e1 l /\ fst e <> fst e1 /\ fst e > fst e1) \/
+                            (mem e (diff a l) /\ mem e1 (diff b l) /\ fst e <> fst e1 /\ fst e > fst e1) \/
+                            (mem e (diff b l) /\ mem e1 (diff a l) /\ fst e <> fst e1 /\ fst e > fst e1)*)))
 
-#set-options "--z3rlimit 10000"
+#set-options "--z3rlimit 10000000"
 let merge ltr l atr a btr b = 
-  merge1 l a b
-
-#set-options "--z3rlimit 1000000"
-val lem_abs : ltr:ae op
-                 -> atr:ae op
-                 -> btr:ae op
-                 -> Lemma (requires (forall e. mem e ltr.l ==> not (member (get_id e) atr.l)) /\
-                                   (forall e. mem e atr.l ==> not (member (get_id e) btr.l)) /\
-                                   (forall e. mem e ltr.l ==> not (member (get_id e) btr.l)) /\
-                                   (forall e e1. mem e ltr.l /\ mem e1 atr.l ==> get_id e < get_id e1) /\
-                                   (forall e e1. mem e ltr.l /\ mem e1 btr.l ==> get_id e < get_id e1))
-                         (ensures (forall e e1. (mem e (absmerge ltr atr btr).l /\ mem e1 (absmerge ltr atr btr).l /\
-                        get_id e <> get_id e1 /\ get_id e > get_id e1 /\ (absmerge ltr atr btr).vis e1 e) <==>
-            (mem e ltr.l /\ mem e1 ltr.l /\ get_id e <> get_id e1 /\ get_id e > get_id e1 /\ ltr.vis e1 e) \/
-            (mem e atr.l /\ mem e1 atr.l /\ get_id e <> get_id e1 /\ get_id e > get_id e1 /\ atr.vis e1 e) \/
-            (mem e btr.l /\ mem e1 btr.l /\ get_id e <> get_id e1 /\ get_id e > get_id e1 /\ btr.vis e1 e) \/
-            (mem e atr.l /\ mem e1 ltr.l /\ get_id e <> get_id e1 /\ get_id e > get_id e1) \/
-            (mem e btr.l /\ mem e1 ltr.l /\ get_id e <> get_id e1 /\ get_id e > get_id e1) \/
-            (mem e atr.l /\ mem e1 btr.l /\ get_id e <> get_id e1 /\ get_id e > get_id e1) \/
-            (mem e btr.l /\ mem e1 atr.l /\ get_id e <> get_id e1 /\ get_id e > get_id e1)))
-            (decreases %[ltr.l;atr.l;btr.l])
-
-#set-options "--z3rlimit 1000000"
-let rec lem_abs ltr atr btr = 
-  (*)match ltr.l,atr.l,btr.l with
-  |[],[],[] -> ()
-  |x::xs,_,_ -> lem_abs (A ltr.vis xs) atr btr
-  |[],x::xs,_ -> lem_abs ltr (A atr.vis xs) btr
-  |[],[],x::xs -> lem_abs ltr atr (A btr.vis xs)*) admit ()
+  assert (forall e. mem e l ==> mem e a /\ mem e b);
+  assert (forall e e1. mem e a /\ not (mem e l) /\ mem e1 b /\ not (mem e1 l) ==> e <> e1);
+  let la = filter (fun e -> not (mem e l)) a in
+  assert (unique_s la /\ total_order la);
+  assert (forall e e1. mem e l /\ mem e1 la ==> fst e1 > fst e);
+  let lb = filter (fun e -> not (mem e l)) b in
+  assert (unique_s lb /\ total_order lb);
+  assert (forall e e1. mem e l /\ mem e1 lb ==> fst e1 > fst e);
+  assert (forall id. mem_id_s id la ==> not (mem_id_s id lb));
+  let u = un la lb in
+  assert (forall id. mem_id_s id l ==> not (mem_id_s id u));
+  assert (forall e e1. mem e l /\ mem e1 u ==> fst e <> fst e1);
+  un u l
 
 val prop_merge : ltr:ae op
                -> l:s
@@ -213,24 +273,24 @@ val prop_merge : ltr:ae op
 
 #set-options "--z3rlimit 10000000"
 let prop_merge ltr l atr a btr b = 
-  lem_abs ltr atr btr;
+  (*)lem_abs ltr atr btr;*)
     assert (forall e. mem e (merge ltr l atr a btr b) <==> mem (fst e, (Append (snd e))) (absmerge ltr atr btr).l);
     assert (forall e e1. mem e (merge ltr l atr a btr b) /\ mem e1 (merge ltr l atr a btr b) /\ fst e <> fst e1 /\ 
                 fst e > fst e1 /\ ord e e1 (merge ltr l atr a btr b) ==>
                 mem (fst e, (Append (snd e))) (absmerge ltr atr btr).l /\ 
                 mem (fst e1, (Append (snd e1))) (absmerge ltr atr btr).l /\
-                fst e <> fst e1 /\ fst e > fst e1 /\ 
-                ((absmerge ltr atr btr).vis (fst e1, (Append (snd e1))) (fst e, (Append (snd e))) ||
+                fst e <> fst e1 /\ fst e > fst e1 (*)/\ 
+                ((absmerge ltr atr btr).vis (fst e1, (Append (snd e1))) (fst e, (Append (snd e))) \/
                   not ((absmerge ltr atr btr).vis (fst e1, (Append (snd e1))) (fst e, (Append (snd e))) ||
-                    (absmerge ltr atr btr).vis (fst e, (Append (snd e))) (fst e1, (Append (snd e1))))));
+                    (absmerge ltr atr btr).vis (fst e, (Append (snd e))) (fst e1, (Append (snd e1))))*));
     assert (forall e e1. mem e (absmerge ltr atr btr).l /\ mem e1 (absmerge ltr atr btr).l /\ get_id e <> get_id e1 /\ 
-                    get_id e > get_id e1 /\ ((absmerge ltr atr btr).vis e1 e ||
-                           not ((absmerge ltr atr btr).vis e e1 || (absmerge ltr atr btr).vis e1 e)) ==> 
+                    get_id e > get_id e1 (*)/\ ((absmerge ltr atr btr).vis e1 e \/
+                           not ((absmerge ltr atr btr).vis e e1 || (absmerge ltr atr btr).vis e1 e)*) ==> 
                       mem (get_id e, get_msg e) (merge ltr l atr a btr b) /\ 
                         mem (get_id e1, get_msg e1) (merge ltr l atr a btr b) /\
              get_id e <> get_id e1 /\ get_id e > get_id e1 /\ 
              ord (get_id e, get_msg e) (get_id e1, get_msg e1) (merge ltr l atr a btr b)); (*done*)
-            admit  ()
+    ()
 
 (*)instance _ : mrdt s op log = {
   Library.merge = merge;
